pcuic/theories/PCUICClosed.v
@@ -727,28 +727,28 @@ Proof.
       rewrite arities_context_length in Hs.
       eauto using closed_upwards with arith.
 
-  - destruct H3 as [clret _].
-    destruct H6 as [clc clty].
+  - destruct H4 as [clret _].
+    destruct H7 as [clc clty].
     rewrite closedn_mkApps in clty. simpl in clty.
     rewrite forallb_app in clty. move/andP: clty => [clpar clinds].
     rewrite app_context_length in clret.
-    red in H8. eapply Forall2_All2 in H8.
+    red in H9. eapply Forall2_All2 in H9.
     eapply All2i_All2_mix_left in X5; eauto.
     intuition auto. 
     + unfold test_predicate_k. simpl. rtoProp; eauto.
       rewrite (case_predicate_context_length H1) in clret; repeat split; tas.
-      rewrite closedn_ctx_app in H2.
-      now move/andP: H2 => [].
-    + unfold test_branch_k. clear H8. solve_all.
+      rewrite closedn_ctx_app in H3.
+      now move/andP: H3 => [].
+    + unfold test_branch_k. clear H9. solve_all.
       * rewrite closedn_ctx_app in a1.
         now move/andP: a1 => [].
       * eapply All2_fold_app_inv_l in b as [_ conv] => //.
-        len in H8.
+        len in H9.
         now rewrite (All2_fold_length conv).
     + rewrite closedn_mkApps; auto.
       rewrite closedn_it_mkLambda_or_LetIn //.
-      rewrite closedn_ctx_app in H4.
-      now move/andP: H4 => [].
+      rewrite closedn_ctx_app in H5.
+      now move/andP: H5 => [].
       now rewrite Nat.add_comm.
       rewrite forallb_app. simpl. now rewrite clc clinds.
 
