pcuic/theories/PCUICValidity.v
@@ -16,6 +16,8 @@ Require Import ssreflect ssrbool.
 
 Derive Signature for typing cumul.
 
+Implicit Types (cf : checker_flags) (Σ : global_env_ext).
+
 Arguments Nat.sub : simpl never.
 
 Section Validity.
@@ -175,21 +177,6 @@ Section Validity.
     induction 1; constructor; auto.
   Qed.
 
-  Lemma case_predicate_context_eq ci mdecl idecl p :
-    wf_predicate mdecl idecl p ->
-    eq_context_upto_names (case_predicate_context ci mdecl idecl p)
-      (case_predicate_binder idecl ci p :: 
-        subst_context (pparams p) 0 (subst_instance p.(puinst) 
-          (expand_lets_ctx (ind_params mdecl) (ind_indices idecl)))).
-  Proof.
-    intros [].
-    rewrite /case_predicate_context /case_predicate_context_gen.
-    eapply Forall2_All2 in H0.
-    eapply All2_fold_All2.
-    eapply All2_map2_left_All3.
-    todo "cases".
-  Admitted.
-
   Lemma map2_app {A B C} (f : A -> B -> C) l0 l0' l1 l1' :
     #|l0| = #|l1| -> #|l0'| = #|l1'| ->
     map2 f (l0 ++ l0') (l1 ++ l1') = 
@@ -245,6 +232,19 @@ Section Validity.
         subst_context_length lift_context_length.
         constructor. simpl. simpl in H. now noconf H.
         eapply IHX. simpl in H. now noconf H.
+  Qed.
+
+  Lemma wf_pre_case_predicate_context_gen {ci mdecl idecl} {p} :
+    wf_predicate mdecl idecl p ->
+    All2 (fun (x : binder_annot name) (y : context_decl) => eq_binder_annot x (decl_name y))
+      (forget_types (pcontext p)) 
+      (pre_case_predicate_context_gen ci mdecl idecl (pparams p) (puinst p)).
+  Proof.
+    move=> [] hlen /Forall2_All2. rewrite /pre_case_predicate_context_gen.
+    intros a; depind a. rewrite H.
+    constructor. simpl. now simpl in r.
+    clear -a.
+    now eapply All2_eq_binder_subst_context_inst.
   Qed.
 
   Theorem validity_env :
@@ -346,135 +346,23 @@ Section Validity.
       rewrite /ptm. exists ps. red.
       eapply type_mkApps; eauto.
       eapply type_it_mkLambda_or_LetIn; tea.
-      rewrite subst_instance_app_ctx in X7.
-      rewrite smash_context_app_expand in X7.
-      eapply spine_subst_app_inv in X7; eauto.
-      2:{ rewrite context_assumptions_smash_context /=.
-          len. pose proof (wf_predicate_length_pars H0).
-          rewrite H. symmetry. apply onmind.(onNpars). }
-      rewrite expand_lets_ctx_length smash_context_length /= 
-        context_assumptions_subst_instance
-        in X7.
-      destruct X7 as [sppars spidx].
-      assert (lenidx : context_assumptions (ind_indices idecl) = #|indices|).
-      { pose proof (PCUICContextSubst.context_subst_length2 spidx).
-        len in H. rewrite context_assumptions_smash_context in H. now len in H. }
-      assert (lenpars : context_assumptions (ind_params mdecl) = #|pparams p|).
-      { pose proof (PCUICContextSubst.context_subst_length2 sppars).
-        now rewrite context_assumptions_smash_context in H; len in H. }
-      assert (firstn (context_assumptions (ind_indices idecl))
-           (List.rev (pparams p ++ indices)) = List.rev indices).
-      { rewrite List.rev_app_distr.
-        now rewrite (firstn_app_left _ 0); 
-        rewrite /= ?app_nil_r // Nat.add_0_r List.rev_length. }
-      assert (skipn (context_assumptions (ind_indices idecl))
-        (List.rev (pparams p ++ indices)) = List.rev (pparams p)).
-      { rewrite List.rev_app_distr.
-        erewrite (skipn_all_app_eq) => //; rewrite List.rev_length //. }        
-      rewrite H H2 in spidx, sppars.
-
-      eapply typing_spine_strengthen. tea.
+      eapply typing_spine_strengthen; tea.
       2:{ rewrite /predctx /= /case_predicate_context /case_predicate_context_gen. 
-        constructor.
-        eapply PCUICEquality.eq_term_leq_term.
-        eapply eq_term_set_binder_name.
-        destruct H0. eapply Forall2_All2 in H4.
-        move: H4. clear.
-        intros a; depind a. rewrite H.
-        constructor. simpl. now simpl in r.
-        clear -a.
-        now eapply All2_eq_binder_subst_context_inst. }
+          constructor.
+          eapply PCUICEquality.eq_term_leq_term.
+          eapply eq_term_set_binder_name.
+          now eapply wf_pre_case_predicate_context_gen. }
+      rewrite /pre_case_predicate_context_gen.
       set (iass := {| decl_name := _ |}).
-      rewrite subst_instance_expand_lets_ctx.
       eapply wf_arity_spine_typing_spine; auto.
+      rewrite subst_instance_app_ctx in X7.
+      eapply spine_subst_smash_app_inv in X7 as [sppars spidx].
+      2:{ rewrite (wf_predicate_length_pars H0). len.
+          now rewrite onmind.(onNpars). }
       split; auto.
-      * (* We show that the derived predicate is well-typed, along with its application 
-           to the discriminee's indices *)
-        unshelve epose proof (on_inductive_inst isdecl _ _ _ cu). 2:tea.
-        rewrite -/(subst_context_let_expand _ _ _).
-        rewrite subst_instance_app_ctx in X7.
-        destruct X7 as [s Hs]. red in Hs.
-        eapply isType_it_mkProd_or_LetIn_app in Hs. 2:eapply sppars.
-        rewrite subst_let_expand_it_mkProd_or_LetIn in Hs.
-        eapply type_it_mkProd_or_LetIn_inv in Hs as (idxs & inds & sortsidx & sortind & leq).
-        eexists (sort_of_products (subst_instance (puinst p) (ind_sort idecl) :: idxs)
-          (Universe.super ps)); red.
-        set (idxctx := subst_context_let_expand _ _ _) in *.
-        have tyass : Σ ;;; Γ ,,, idxctx |- decl_type iass : 
-          tSort (subst_instance (puinst p) (ind_sort idecl)).
-        { pose proof (on_inductive_sort_inst isdecl _ cu).
-          rewrite /iass /=.
-          have wfidxctx : wf_local Σ (Γ ,,, idxctx) by pcuic.
-          eapply pre_type_mkApps_arity. econstructor; tea. pcuic.
-          eapply on_inductive_isType; tea. pcuic.
-          rewrite oib.(ind_arity_eq) subst_instance_it_mkProd_or_LetIn.
-          eapply arity_spine_it_mkProd_or_LetIn_smash; tea.
-          rewrite -[smash_context [] _](closed_ctx_lift #|idecl.(ind_indices)| 0).
-          { eapply closedn_smash_context.
-            rewrite closedn_subst_instance_context.
-            eapply (declared_inductive_closed_params isdecl). }
-          relativize #|ind_indices idecl|.
-          rewrite -map_rev. eapply subslet_lift; tea.
-          eapply sppars. now rewrite /idxctx; len.
-          rewrite subst_instance_it_mkProd_or_LetIn subst_let_expand_it_mkProd_or_LetIn /=.
-          eapply arity_spine_it_mkProd_or_LetIn_Sort => //. reflexivity.
-          relativize (subst_context_let_expand (List.rev (map _ _)) _ _).
-          relativize (to_extended_list _).
-          eapply spine_subst_to_extended_list_k; tea.
-          rewrite [reln [] _ _]to_extended_list_subst_context_let_expand.
-          apply PCUICLiftSubst.map_subst_instance_to_extended_list_k.
-          rewrite subst_context_let_expand_length subst_instance_length.
-          rewrite /subst_context_let_expand.
-          rewrite distr_lift_subst_context map_rev. f_equal.
-          rewrite List.rev_length Nat.add_0_r.
-          rewrite PCUICClosed.closed_ctx_lift //.
-          rewrite -lenpars.
-          relativize (context_assumptions _).
-          eapply closedn_ctx_expand_lets.
-          rewrite -subst_instance_app_ctx closedn_subst_instance_context.
-          eapply (declared_inductive_closed_pars_indices _ isdecl). now len. }  
-        eapply type_it_mkProd_or_LetIn_sorts; tea.
-        constructor => //.
-        constructor => //. simpl.
-        constructor => //.
-        now eapply sorts_local_ctx_wf_local; tea. red.
-        eexists; tea. 
-        now eapply typing_wf_universe in IHp.
-      * simpl. eapply arity_spine_it_mkProd_or_LetIn_smash; tea.
-        rewrite (smash_context_subst []).
-        rewrite (expand_lets_smash_context _ []) 
-          expand_lets_k_ctx_nil /= in spidx.
-        apply spidx. rewrite subst_let_expand_tProd.
-        constructor.
-        2:econstructor.
-        set (ictx := subst_instance (puinst p) _).
-        eapply meta_conv; tea.
-        rewrite subst_let_expand_mkApps subst_let_expand_tInd map_app.
-        f_equal. f_equal.
-        rewrite -{1}[pparams p](map_id (pparams p)).
-        rewrite map_map_compose; eapply map_ext => x.
-        setoid_rewrite subst_let_expand_lift_id; auto.
-        now rewrite /ictx; len.
-        rewrite /ictx /expand_lets_ctx /expand_lets_k_ctx; len.
-        now symmetry.
-        (* Should be a lemma *)
-        rewrite -subst_context_map_subst_expand_lets.
-        now rewrite /ictx; len. 
-        rewrite /subst_let_expand /expand_lets /expand_lets_k.
-        rewrite -map_map_compose.
-        rewrite -{1}(spine_subst_subst_to_extended_list_k spidx).
-        f_equal.
-        rewrite to_extended_list_k_subst /expand_lets_ctx /expand_lets_k_ctx.
-        rewrite !to_extended_list_k_subst to_extended_list_k_lift_context.
-        rewrite -map_map_compose. simpl. len.
-        rewrite lift_to_extended_list_k.
-        set (ctx := subst_context _ _ _).
-        assert (to_extended_list_k (ind_indices idecl) 0 = to_extended_list_k ctx 0) as ->.
-        { rewrite /ctx to_extended_list_k_subst.
-          now rewrite PCUICLiftSubst.map_subst_instance_to_extended_list_k. }
-        rewrite extended_subst_to_extended_list_k /ctx.
-        now rewrite (smash_context_subst []) to_extended_list_k_subst.
-        
+      * eapply isType_case_predicate => //; pcuic.
+      * eapply arity_spine_case_predicate => //; pcuic.
+
     - (* Proj *)
       pose proof isdecl as isdecl'.
       eapply declared_projection_type in isdecl'; eauto.
@@ -517,14 +405,14 @@ Section Validity.
 
 End Validity.
 
-Corollary validity {cf:checker_flags} {Σ Γ t T} :
-  wf Σ.1 -> Σ ;;; Γ |- t : T -> isType Σ Γ T.
+Corollary validity {cf:checker_flags} {Σ} {wfΣ : wf Σ} {Γ t T} :
+  Σ ;;; Γ |- t : T -> isType Σ Γ T.
 Proof.
   intros. eapply validity_env; try eassumption.
 Defined.
 
 (* To deprecate *)
-Notation validity_term := validity.
+Notation validity_term wf Ht := (validity (wfΣ:=wf) Ht).
 
 (* This corollary relies strongly on validity to ensure 
    every type in the derivation is well-typed.
@@ -563,6 +451,18 @@ Lemma type_App' {cf:checker_flags} {Σ : global_env_ext} {wfΣ : wf Σ} {Γ t na
   Σ;;; Γ |- u : A -> Σ;;; Γ |- tApp t u : B {0 := u}.
 Proof.
   intros Ht Hu.
-  have [s Hs] := validity wfΣ Ht.
+  have [s Hs] := validity Ht.
   eapply type_App; eauto.
+Qed.
+
+Lemma type_mkApps_arity {cf} {Σ : global_env_ext} {wfΣ : wf Σ} {Γ t u tty T} :
+  Σ;;; Γ |- t : tty ->
+  arity_spine Σ Γ tty u T -> 
+  Σ;;; Γ |- mkApps t u : T.
+Proof.
+  intros Ht Hty.
+  pose proof (validity Ht).
+  eapply type_mkApps; tea.
+  eapply wf_arity_spine_typing_spine; tea.
+  constructor; tas.
 Qed.
